commit

AP/Paramodulator/Defs.lean
@@ -13,13 +13,33 @@ declare_syntax_cat node
 
 syntax num : node
 syntax ident : node
-syntax "(" node node ")" : node
+syntax node node : node
+syntax "(" node ")" : node
 syntax "!!" node : term
 
 macro_rules
-  | `(!!($a:node $b:node)) => `(pair (!!$a) (!!$b))
+  | `(!!$a:node $b:node) => `(pair (!!$a) (!!$b))
+  | `(!!($a:node)) => `(!!$a)
   | `(!!$a:num) => `($a)
   | `(!!$a:ident) => `($a)
 
 instance : Zero Node := ⟨nil⟩
 instance : One Node := ⟨!!(0 0)⟩
+
+@[simp]
+def const (n : ℕ) : Node :=
+  match n with
+  | 0 => 1
+  | n + 1 => pair 0 # const n
+
+@[simp]
+def Node.left (x : Node) : Node :=
+  match x with
+  | .pair x _ => x
+  | _ => 0
+
+@[simp]
+def Node.right (x : Node) : Node :=
+  match x with
+  | .pair _ y => y
+  | _ => 0
