AP/Paramodulator/Main.lean
@@ -1,3 +1,4 @@
 import AP.Paramodulator.Defs
 import AP.Paramodulator.Basic
 import AP.Paramodulator.Systems
+import AP.Paramodulator.Nat
