AP/Paramodulator/Systems.lean
@@ -1,3 +1,4 @@
 import AP.Paramodulator.Systems.S_21
 import AP.Paramodulator.Systems.S_24
 import AP.Paramodulator.Systems.S_32
+import AP.Paramodulator.Systems.S_61
