AP/Paramodulator/Systems/S_61.lean
@@ -1,0 +1,34 @@
+import AP.Paramodulator.Basic
+
+namespace Paramodulator.S_61
+
+open Node
+
+instance : OfNat Node 2 := ⟨!!(1 0)⟩
+theorem n2_def : (2 : Node) = !!(1 0) := rfl
+
+instance : OfNat Node 3 := ⟨!!(2 1)⟩
+theorem n3_def : (3 : Node) = !!(2 1) := rfl
+
+inductive P : Node → Prop where
+| r0 : P (!!(2 1))
+| r1 {a} : P a → P (!!((a 0) 3))
+| r2 {a b} : P (!!(1 a)) → P b → P a
+
+-----
+
+inductive P' : Node → Prop where
+| r0 : P' 3
+| r1 {a} : P' a → P' (!!((a 0) 3))
+
+-----
+
+theorem p_eq_p' : P = P' := by
+  ext a; constructor <;> intro h
+  · induction h
+    · exact P'.r0
+    · nm x h ih; exact P'.r1 ih
+    · nm x y h₁ h₂ ih₁ ih₂; cases ih₁; nm h₃; cases h₃
+  · induction h
+    · exact P.r0
+    · nm x h ih; exact P.r1 ih
